examples/steel/Duplex.PCM.fsti
@@ -1,0 +1,89 @@
+module Duplex.PCM
+open FStar.PCM
+open Steel.Memory
+open Steel.Effect.Atomic
+open Steel.Effect
+open Steel.Channel.Protocol
+
+let dprot' = protocol unit
+
+module P = FStar.Preorder
+module R = FStar.ReflexiveTransitiveClosure
+
+// Simplifying protocols for now
+let rec no_loop (p:protocol 'a) =
+  match p with
+  | Return _ -> True
+  | Msg _ a k -> (forall x. no_loop (k x))
+  | DoWhile _ _ -> False
+
+let dprot = p:dprot'{no_loop p}
+
+let nl_protocol 'a = p:protocol 'a { no_loop p }
+let return (#a:_) (x:a) : nl_protocol a = Return x
+let done : dprot = return ()
+let send a : nl_protocol a = Msg Send a return
+let recv a : nl_protocol a = Msg Recv a return
+let rec bind #a #b (p:nl_protocol a) (q:(a -> nl_protocol b))
+  : nl_protocol b
+  = match p with
+    | Return v -> q v
+    | Msg tag c #a' k ->
+       let k : c -> nl_protocol b =
+        fun x -> bind (k x) q
+      in
+      Msg tag c k
+
+////////////////////////////////////////////////////////////////////////////////
+
+type party = | A | B
+
+type send_next_dprot_t (name:party) =
+  next:dprot{more next /\ tag_of next == (if name = A then Send else Recv)}
+
+type recv_next_dprot_t (name:party) =
+  next:dprot{more next /\ tag_of next == (if name = A then Recv else Send)}
+
+val channel (p:dprot) : Type0
+
+val endpt (#p:dprot) (name:party) (c:channel p) (next:dprot) : slprop u#1
+
+val new_channel (p:dprot)
+  : SteelT (channel p & channel p) emp
+           (fun cc -> endpt A (fst cc) p `star` endpt B (snd cc) p)
+
+val channel_send (#name:party)
+         (#p:dprot)
+         (#next:send_next_dprot_t name)
+         (c:channel p) (x:msg_t next)
+  : SteelT unit
+      (endpt name c next)
+      (fun _ -> endpt name c (step next x))
+
+val channel_recv (#name:party)
+         (#p:dprot)
+         (#next:recv_next_dprot_t name)
+         (c:channel p)
+  : SteelT (msg_t next)
+      (endpt name c next)
+      (fun x -> endpt name c (step next x))
+
+////////////////////////////////////////////////////////////////////////////////
+// An example
+////////////////////////////////////////////////////////////////////////////////
+
+let pingpong : dprot =
+  x <-- send int;
+  y <-- recv (y:int{y > x});
+  done
+
+let client (c:channel pingpong)
+  : SteelT unit
+           (endpt A c pingpong)
+           (fun _ -> endpt A c done)
+  = // In this implementation, the client first sends the (arbitrarily chosen) integer 17
+    channel_send #A c 17;
+    let y = channel_recv #A c in
+    // The protocol specifies that the integer received is greater than the one sent.
+    // This fact is available in the context and can be asserted.
+    assert (y > 17)
